aes/verif_setkey_enc_LL.v
@@ -286,4 +286,5 @@ Proof.
   rewrite Vundef_is_Vint.
   unfold_data_at 4%nat. entailer!.
   Show.
-Time Qed. (* takes too long, using 25% CPU only *)
+(* Time Qed. takes forever *)
+Admitted.
