Makefile
@@ -328,10 +328,9 @@ HMACDRBG_FILES = \
   verif_hmac_drbg_generate.v verif_hmac_drbg_seed_buf.v verif_mocked_md.v \
   verif_hmac_drbg_seed.v verif_hmac_drbg_NISTseed.v verif_hmac_drbg_other.v
 
+# these are only the top-level AES files, but they depend on many other AES files, so first run "make depend"
 AES_FILES = \
-  aes.v sbox.v tablesLL.v \
-  verif_encryption_ll.v \
-  AES256.v aes_round_lemmas.v aesutils.v forwarding_table_lemmas.v mult_equiv_lemmas.v verif_aes256.v
+  verif_encryption_LL.v verif_gen_tables_LL.v verif_setkey_enc_LL.v equiv_encryption.v
 
 # DRBG_Files = \
 #  hmac_drbg.v HMAC256_DRBG_functional_prog.v hmac_drbg_compspecs.v \
